Add call semantics

theories/clang/lang.v
@@ -182,6 +182,9 @@ Fixpoint storebytes l bs (σ: heap) :=
     | _ => σ
   end.
 
+Definition alloc_heap (l: addr) (v: val) (σ: state) : state :=
+  State (storebytes l (encode_val v) (s_heap σ)) (s_text σ).
+
 (* expr *can* have side-effect *)
 Inductive estep : expr → state → expr → state → Prop :=
 | ESbinop: ∀ lv rv op σ v',
@@ -205,17 +208,7 @@ Inductive estep : expr → state → expr → state → Prop :=
       typeof v t →
       (∀ o', (s_heap σ) !! (b, o') = None) →
       estep (Ealloc t (Evalue v)) σ (Evalue (Vptr (b, o)))
-            (State (storebytes (b, o) (encode_val v) (s_heap σ)) (s_text σ)).
-(* | EScall: *)
-(*     ∀ t v σ  *)
-(*     es = map Evalue vs → *)
-(*     params_match params vs → *)
-(*     (∀ ls f_body', *)
-(*        ⌜ length ls = length vs ∧ *)
-(*          instantiate_f_body (add_params_to_env ev params ls) f_body = Some f_body' ⌝ -∗ *)
-(*        alloc_params (zip (params.*2) ls) vs -∗ *)
-(*        WP curs f_body' {{ _, True; Φ }}) *)
-(*     ⊢ WP cure (Ecall f es) {{ Φ; Φret }}. *)
+            (alloc_heap (b, o) v σ).
 
 (* Offset is ignored *)
 Inductive sstep : stmts → state → stmts → state → Prop :=
@@ -285,9 +278,131 @@ Proof. intros ?. destruct c as [[]|[]]=>//. Qed.
 
 (* Definition of_val (v: val) := Evalue v. *)
 
+Fixpoint params_match (params: decls) (vs: list val) :=
+  match params, vs with
+    | (_, t)::params, v::vs => typeof v t ∧ params_match params vs
+    | [], [] => True
+    | _, _ => False
+  end.
+
+
+Fixpoint lift_list_option {A} (l: list (option A)): option (list A) :=
+  match l with
+    | Some x :: l' => (x ::) <$> lift_list_option l'
+    | None :: _ => None
+    | _ => Some []
+  end.
+
+Fixpoint resolve_rhs_e {t: Type} (ev: @env t) (e: expr) : option expr :=
+  match e with
+    | Evar x => (* closed-ness? *)
+      (match sget x (lenv ev) with
+         | Some (t, l) => Some $ Ederef_typed t (Evalue (Vptr l))
+         | None => None
+       end)
+    | Ebinop op e1 e2 =>
+      match resolve_rhs_e ev e1, resolve_rhs_e ev e2 with
+        | Some e1', Some e2' => Some (Ebinop op e1' e2')
+        | _, _ => None
+      end
+    | Ederef e =>
+      match type_infer ev e, resolve_rhs_e ev e with
+        | Some (Tptr t), Some e' => Some (Ederef_typed t e') 
+        | _, _ => None
+      end
+    | Eaddrof e => Eaddrof <$> resolve_rhs_e ev e
+    | Efst e => Efst <$> resolve_rhs_e ev e
+    | Esnd e => Esnd <$> resolve_rhs_e ev e
+    | Ecall f args => Ecall f <$> lift_list_option (map (resolve_rhs_e ev) args)
+    | _ => Some e
+  end.
+
+Fixpoint resolve_rhs {t: Type} (ev: @env t) (s: stmts) : option stmts :=
+  match s with
+    | Sskip => Some Sskip
+    | Sprim p => Some $ Sprim p
+    | Sassign e1 e2 => Sassign e1 <$> resolve_rhs_e ev e2
+    | Sif e s1 s2 =>
+      match resolve_rhs_e ev e, resolve_rhs ev s1, resolve_rhs ev s2 with
+        | Some e', Some s1', Some s2' => Some $ Sif e' s1' s2'
+        | _, _, _ => None
+      end
+    | Swhile c e s =>
+      match resolve_rhs_e ev c, resolve_rhs_e ev e, resolve_rhs ev s with
+        | Some c', Some e', Some s' => Some $ Swhile c' e' s'
+        | _, _, _ => None
+      end
+    | Srete e => Srete <$> resolve_rhs_e ev e
+    | Sret => Some Sret
+    | Sseq s1 s2 =>
+      match resolve_rhs ev s1, resolve_rhs ev s2 with
+        | Some s1', Some s2' => Some (Sseq s1' s2')
+        | _, _ => None
+      end
+  end.
+
+Fixpoint resolve_lhs_e {t: Type} (ev: @env t) (e: expr) : option expr :=
+  match e with
+    | Evar x =>
+      (match sget x (lenv ev) with
+         | Some (_, l) => Some (Evalue (Vptr l))
+         | None => None
+       end)
+    | Ederef e' => resolve_rhs_e ev e'
+    | Efst e' => resolve_lhs_e ev e'
+    | Esnd e' =>
+      (e'' ← resolve_lhs_e ev e';
+       match type_infer ev e'' with
+         | Some (Tptr (Tprod t1 _)) =>
+           Some (Ebinop oplus e'' (Evalue (Vint8 (Byte.repr (sizeof t1)))))
+         | _ => None
+       end)
+    | Evalue (Vptr l) => Some e
+    | Ecall f es => Some $ Ecall f es
+    | _ => None
+  end.
+
+Fixpoint resolve_lhs {t: Type} (e: @env t) (s: stmts) : option stmts :=
+  match s with
+    | Sassign e1 e2 => e'' ← resolve_lhs_e e e1; Some (Sassign e'' e2)
+    | Sif ex s1 s2 =>
+      match resolve_lhs e s1, resolve_lhs e s2 with
+        | Some s1', Some s2' => Some (Sif ex s1' s2')
+        | _, _ => None
+      end
+    | Swhile c ex s => Swhile c ex <$> resolve_lhs e s
+    | Sseq s1 s2 =>
+      match resolve_lhs e s1, resolve_lhs e s2 with
+        | Some s1', Some s2' => Some (Sseq s1' s2')
+        | _, _ => None
+      end
+    | Sret => Some Sret
+    | Srete e => Some (Srete e)
+    | Sprim p => Some $ Sprim p
+    | Sskip => Some Sskip
+  end.
+
+Fixpoint add_params_to_env {t: Type} (e: @env t) (params: list (ident * type)) ls : env :=
+  match params, ls with
+    | (x, t)::ps, l::ls' => add_params_to_env (Env _ (sset x (t, l) (lenv e)) (fenv e)) ps ls'
+    | _, _ => e
+  end.
+
+Definition instantiate_f_body {t: Type} (ev: @env t) (s: stmts) : option stmts :=
+  (resolve_rhs ev s ≫= resolve_lhs ev).
+
 Inductive cstep: cureval → state → list context → cureval → state → list context → Prop :=
 | CSestep: ∀ e e' σ σ' ks, estep e σ e' σ' → cstep (cure e) σ ks (cure e') σ' ks
-| CSsstep: ∀ s s' σ σ' ks, sstep s σ s' σ' → cstep (curs s) σ ks (curs s') σ' ks.
+| CSsstep: ∀ s s' σ σ' ks, sstep s σ s' σ' → cstep (curs s) σ ks (curs s') σ' ks
+| CSecall:
+    ∀ (ev: @env stmts) es vs ls retty params f_body f_body' f ks σ σ',
+      es = map Evalue vs →
+      params_match params vs →
+      length ls = length vs →
+      s_text σ !! f = Some (Function stmts retty params f_body) →
+      instantiate_f_body (add_params_to_env ev params ls) f_body = Some f_body' →
+      σ' = foldr (fun lv σ => alloc_heap (lv.1) (lv.2) σ) σ (zip ls vs) →
+      cstep (cure (Ecall f es)) σ ks (curs f_body') σ' ks.
 
 Lemma fill_step_inv σ σ' ks ks' e c' Kes Ks:
   to_val (cure e) = None →
